Phi_Semantics/PhiSem_Aggregate_Named_Tuple.thy
@@ -231,10 +231,11 @@ print_translation \<open>[
 subsubsection \<open>Properties\<close>
 
 let_\<phi>type Named_Tuple_Field
-  deriving \<open> Semantic_Type T TY
-         \<Longrightarrow> Semantic_Type \<lbrace> SYMBOL_VAR(s): T \<rbrace> (semty_ntup (fmupd s TY fmempty))\<close>
+  deriving \<open> Weak_Semantic_Type T TY
+         \<Longrightarrow> Weak_Semantic_Type \<lbrace> SYMBOL_VAR(s): T \<rbrace> (semty_ntup (fmupd s TY fmempty))\<close>
        and \<open> Semantic_Zero_Val ty T x
          \<Longrightarrow> Semantic_Zero_Val (semty_ntup (fmupd s ty fmempty)) \<lbrace> SYMBOL_VAR(s): T \<rbrace> x \<close>
+       and Inhabited_Type
 
 text \<open>All the reasoning rules below are for semantic properties.
       All reasoning rules for transformations and SL are derived automatically by the above \<open>\<phi>type_def\<close> command\<close>
@@ -264,12 +265,6 @@ lemma Tuple_Field_semty[\<phi>reason %\<phi>sem_type_cut]:
 \<Longrightarrow> Weak_Semantic_Type \<lbrace> SYMBOL_VAR(s): T \<rbrace> (semty_ntup (fmupd s TY fmempty)) \<close>
   unfolding Weak_Semantic_Type_def subset_iff
   by clarsimp blast
-
-lemma Tuple_Field_semty'[\<phi>reason %\<phi>sem_type_cut]:
-  \<open> Semantic_Type T TY
-\<Longrightarrow> Semantic_Type \<lbrace> SYMBOL_VAR(s): T \<rbrace> (semty_ntup (fmupd s TY fmempty)) \<close>
-  unfolding Semantic_Type_def subset_iff
-  by (clarsimp, rule, blast intro: Tuple_Field_semty, blast intro: Named_Tuple_Field.Inhabited_Type)
 
 lemma Tuple_Field_semty2[\<phi>reason %\<phi>sem_type_cut+10]:
   \<open> Weak_Semantic_Type T TY
@@ -334,21 +329,19 @@ lemma [\<phi>reason %chk_sem_ele_idx+20]:
 
 
 lemma [\<phi>reason %\<phi>sem_type_cut+10]:
-  \<open> Semantic_Type T TY
-\<Longrightarrow> Semantic_Type Ts (semty_ntup TYs)
+  \<open> Inhabited_Type T
 \<Longrightarrow> Is_Named_Tuple Ts fields
 \<Longrightarrow> \<c>\<o>\<n>\<d>\<i>\<t>\<i>\<o>\<n> s |\<notin>| fields
-\<Longrightarrow> Semantic_Type (\<lbrace> SYMBOL_VAR(s): T \<rbrace> \<^emph> Ts) (semty_ntup (fmupd s TY TYs))\<close>
-unfolding Semantic_Type_def subset_iff Premise_def
-          Inhabited_Type_def Inhabited_def Weak_Semantic_Type_def Is_Named_Tuple_def
-  apply (clarsimp, rule)
-  apply (metis V_named_tup.dest_mk V_named_tup_mult fmap_times_fempty(2) fmrel_upd fmupd_times_right)
-  subgoal premises prems for x p y q
-    by (insert prems(1)[THEN spec, THEN spec, THEN mp, OF prems(6)],
+\<Longrightarrow> Inhabited_Type Ts
+\<Longrightarrow> Inhabited_Type (\<lbrace> SYMBOL_VAR(s): T \<rbrace> \<^emph> Ts) \<close>
+  unfolding subset_iff Premise_def Inhabited_Type_def Inhabited_def Weak_Semantic_Type_def Is_Named_Tuple_def
+  apply (clarsimp)
+  subgoal premises prems for x y p q
+    by (insert prems(1)[THEN spec, THEN spec, THEN mp, OF prems(4)],
         clarify,
         rule exI[where x=x], rule exI[where x=y],
         rule exI[where x=\<open>V_named_tup.mk (fmupd s p fmempty)\<close>],
-        rule exI[where x=q], insert prems(1-4,6), clarsimp, blast) .
+        rule exI[where x=q], insert prems(2-4), clarsimp, blast) .
 
 
 
